messageInvariantPrototypes/flexPaxos/automate/readme.md
@@ -1,0 +1,4 @@
+# Readme
+
+Monotonic version of Decentralized Paxos with global history.
+This version has templated message invariants, derived from Send Predicated.
